compiler/scheme/scheme_astScript.sml
@@ -12,7 +12,7 @@ Type loc = “:num”
 (* This needs completing: Var, Lit, ... *)
 Datatype:
   prim = SAdd | SMul | SMinus | SEqv | CallCC
-       | Cons | Car | Cdr
+       | Cons | Car | Cdr | IsNull | IsPair
 End
 
 Datatype:
